src/reflection/FStar.Reflection.Embeddings.fsti
@@ -71,3 +71,4 @@ val unfold_lazy_comp   : lazyinfo -> term
 val unfold_lazy_env    : lazyinfo -> term
 val unfold_lazy_sigelt : lazyinfo -> term
 val unfold_lazy_letbinding : lazyinfo -> term
+val unfold_lazy_universe   : lazyinfo -> term
